bedrock2/src/Examples/ipow.v
@@ -1,0 +1,147 @@
+Require Import bedrock2.Macros bedrock2.Syntax.
+Require Import bedrock2.BasicC64Syntax bedrock2.BasicALU bedrock2.NotationsInConstr.
+
+Import BinInt String List.ListNotations.
+Local Open Scope string_scope. Local Open Scope Z_scope. Local Open Scope list_scope.
+Local Existing Instance bedrock2.BasicC64Syntax.Basic_bopnames_params.
+Local Coercion literal (z : Z) : expr := expr.literal z.
+Local Coercion var (x : string) : expr := expr.var x.
+
+Definition ipow := ("ipow", (["x";"e"], (["ret"]:list varname), bedrock_func_body:(
+  "ret" = 1;;
+  while ("e") {{
+    if ("e" .& 1) {{ "ret" = "ret" * "x" }};;
+    "e" = "e" >> 1;;
+    "x" = "x" * "x"
+  }}
+))).
+
+Require Import bedrock2.Semantics bedrock2.BasicC64Semantics bedrock2.Map.
+Require Import bedrock2.Map.Separation bedrock2.Map.SeparationLogic.
+Require bedrock2.WeakestPrecondition bedrock2.WeakestPreconditionProperties.
+Require bedrock2.TailRecursion.
+
+Section WithT.
+  Context {T : Type}.
+  Fixpoint bindcmd (c : cmd) (k : cmd -> T) {struct c} : T :=
+    match c with
+    | cmd.cond e c1 c2 => bindcmd c1 (fun c1 => bindcmd c2 (fun c2 => let c := cmd.cond e c1 c2 in k c))
+    | cmd.seq c1 c2 => bindcmd c1 (fun c1 => bindcmd c2 (fun c2 => let c := cmd.seq c1 c2 in k c))
+    | cmd.while e c => bindcmd c (fun c => let c := cmd.while e c in k c)
+    | c => let c := c in k c
+    end.
+End WithT.
+
+Definition spec_of_ipow := fun functions =>
+  forall x e t m,
+    WeakestPrecondition.call (fun _ => True) (fun _ => False) (fun _ _ => True) functions
+      (fst ipow) t m [x; e]
+      (fun t' m' rets => t=t'/\ m=m' /\ exists v, rets = [v]).
+
+Ltac bind_body_of_function f :=
+  let fname := open_constr:(_) in
+  let fargs := open_constr:(_) in
+  let frets := open_constr:(_) in
+  let fbody := open_constr:(_) in
+  let funif := open_constr:((fname, (fargs, frets, fbody))) in
+  unify f funif;
+  let G := lazymatch goal with |- ?G => G end in
+  let P := lazymatch eval pattern ipow in G with ?P _ => P end in
+  change (bindcmd fbody (fun c : cmd => P (fname, (fargs, frets, c))));
+  cbv beta iota delta [bindcmd]; intros.
+
+Ltac refine_ex :=
+  hnf;
+  let P := lazymatch goal with |- ex ?P => P end in
+  refine (let l := _ in ex_intro P l _).
+
+Ltac refine_ex_and :=
+  hnf;
+  let P := lazymatch goal with |- ex ?P => P end in
+  refine (let l := _ in ex_intro P l (conj _ _)).
+
+Ltac break_ex :=
+  repeat match goal with
+         | H: exists _, _ |- _ => destruct H
+         end.
+
+Ltac subst_and_bind_all :=
+  repeat match goal with
+  | H: ?x = ?v |- _ =>
+    assert_succeeds (subst x);
+    let x' := fresh "x" in rename x into x';
+    simple refine (let x := v in _);
+    replace x' with x by congruence; clear H
+  end.
+
+Lemma ipow_ok : forall functions, spec_of_ipow (ipow::functions).
+Proof.
+  bind_body_of_function ipow.
+  cbv [spec_of_ipow]. intros.
+
+  refine_ex_and.
+  { exact eq_refl. }
+  refine_ex_and.
+  { refine_ex_and.
+    { repeat (refine_ex_and || exact eq_refl). }
+    exact eq_refl. }
+
+  eapply TailRecursion.tailrecursion with
+      (lt:=Z.lt)
+      (P:=fun _ _ l _ => exists x e ret, l = (map.put (map.put (map.put map.empty "x" x) "e" e) "ret" ret))
+      (Q:=fun _ _ l _ => exists x e ret, l = (map.put (map.put (map.put map.empty "x" x) "e" e) "ret" ret))
+      (R0 := fun m' => m'=m).
+  admit.
+  admit.
+  admit.
+  intros.
+
+  (* TODO: lemma for destructing [sep emp _] hyps *) destruct H as (?&?&?&?&?).
+
+  break_ex.
+  subst_and_bind_all.
+
+  refine_ex_and.
+  { repeat (refine_ex_and || exact eq_refl). }
+  split; intros.
+  { refine_ex_and.
+    { repeat (refine_ex_and || exact eq_refl). }
+    split; intros.
+    { refine_ex_and.
+      { repeat (refine_ex_and || exact eq_refl). }
+      refine_ex_and.
+      { repeat (refine_ex_and || exact eq_refl). }
+      refine_ex_and.
+      { repeat (refine_ex_and || exact eq_refl). }
+      eexists. eexists. split.
+      { assert (exists x6 e0 ret : word,
+       map.put (map.put (map.put l1 "ret" l5) "e" l6) "x" l =
+       map.put (map.put (map.put map.empty "x" x6) "e" e0) "ret" ret); [|admit].
+       { do 3 eexists. exact eq_refl. } }
+      { split.
+        { admit. }
+        { admit. } } }
+    { refine_ex_and.
+      { repeat (refine_ex_and || exact eq_refl). }
+      refine_ex_and.
+      { repeat (refine_ex_and || exact eq_refl). }
+      eexists. eexists. split.
+      { assert (exists x6 e0 ret : word,
+       map.put (map.put l1 "e" l5) "x" l =
+       map.put (map.put (map.put map.empty "x" x6) "e" e0) "ret" ret); [|admit].
+       { do 3 eexists. exact eq_refl. } }
+      { split.
+        { admit. }
+        { admit. } } } }
+  { admit. (* TODO: make sure emp actually enforces that mem is empty *) }
+  intros.
+  (* TODO: lemma for destructing [sep emp _] hyps *) destruct H as (?&?&?&?&?).
+  break_ex.
+  subst_and_bind_all.
+  refine_ex_and.
+  { repeat (refine_ex_and || exact eq_refl). }
+  repeat eexists.
+  admit. (* TODO: thread through t=t0 *)
+  admit. (* TODO: thread through m=m0 *)
+  Fail idtac.
+Abort.
